tactics: fix Neg exmple

examples/tactics/Neg.fst
@@ -14,9 +14,8 @@ let  xi = squash __xi
 assume val c1 : unit -> ST unit (requires (fun h0 -> phi)) (ensures (fun h0 () h1 -> psi))
 assume val c2 : unit -> ST unit (requires (fun h0 -> psi)) (ensures (fun h0 () h1 ->  xi))
 
-// by_tactic appears in a double negative position
-val c3 : unit -> ST unit (requires (fun h0 -> phi)) (ensures (fun h0 () h1 -> by_tactic idtac xi))
-let c3 () = c1 (); c2 ()
+val c3 : unit -> ST unit (requires (fun h0 -> phi)) (ensures (fun h0 () h1 -> xi))
+let c3 () = c1 (); c2 (); assert_by_tactic idtac xi
 
 // by_tactic is in negative position, should be peeled off!
 val c4 : unit -> ST unit (requires (fun h0 -> phi)) (ensures (fun h0 () h1 -> xi))
